src/opt/ReorderUpdate.v
@@ -128,7 +128,7 @@ Proof.
     - eapply TView.future_closed; eauto. apply WF2.
     - inv READ. apply WF_SRC.
     - apply WF2.
-    - eapply Memory.future_half_wf; eauto. apply WF2.
+    - eapply Memory.future_reserve_wf; eauto. apply WF2.
   }
   i. des.
   econs; [eauto|..]; s; eauto; etrans; eauto.
@@ -180,7 +180,7 @@ Proof.
     - eapply TView.future_closed; eauto. apply WF2.
     - inv READ. ss. apply WF.
     - apply WF2.
-    - eapply Memory.future_half_wf; eauto. apply WF2.
+    - eapply Memory.future_reserve_wf; eauto. apply WF2.
   }
   i. des.
   exploit sim_local_fulfill_bot; try exact x1; try exact LOCAL0; try refl; eauto.
@@ -189,7 +189,7 @@ Proof.
     - eapply TView.future_closed; eauto. apply WF2.
     - inv READ. apply WF.
     - apply WF2.
-    - eapply Memory.future_half_wf; eauto. apply WF2.
+    - eapply Memory.future_reserve_wf; eauto. apply WF2.
   }
   i. des.
   exploit fulfill_step_future; eauto. i. des.
@@ -485,7 +485,7 @@ Proof.
       exploit Thread.rtc_tau_step_future; eauto. s. i. des.
       exploit Thread.opt_step_future; eauto. s. i. des.
       exploit Thread.program_step_future; eauto. s. i. des.
-      hexploit Thread.step_bot_no_half; [econs 2; eauto|..]; eauto. s. i. des.
+      hexploit Thread.step_bot_no_reserve; [econs 2; eauto|..]; eauto. s. i. des.
       punfold SIM. exploit SIM; try apply SC3; eauto; try refl. s. i. des.
       exploit PROMISES; eauto. i. des.
       * left.
